HelloWorld.thy
@@ -3,7 +3,7 @@ theory HelloWorld
     "~~/src/HOL/Library/Code_Char" (*must be loaded at the end*)
 begin
 
-  text\<open>The main function, defined in Isabelle. It should have the right type in Haskell.\<close>
+text\<open>The main function, defined in Isabelle. It should have the right type in Haskell.\<close>
 definition main :: "unit IO" where
   "main \<equiv> do {
                _ \<leftarrow> println (String.implode ''Hello World!'');
@@ -23,5 +23,6 @@ export_code main in SML file "code/main.sml"
 (*
   $ LD_PRELOAD=~/bin/Isabelle2016-1/contrib/polyml-5.6-1/x86-linux/libgmp.so.3 \
     ~/bin/Isabelle2016-1/contrib/polyml-5.6-1/x86-linux/poly --use main.sml
+  Loads a interpreter and executes main during this. Hacky.
 *)
 end
